Foundation/FirstOrder/Arithmetic/Basic/Hierarchy.lean
@@ -412,6 +412,22 @@ lemma remove_exists {φ : Semiformula L ξ (n + 1)} : Hierarchy b s (∃¹ φ) �
   |     0 => simp
   | k + 1 => simp [LO.FirstOrder.allItr_succ, allItr]
 
+lemma quantItr {φ : Semiformula L ξ (n + s)}
+    (h : Hierarchy (Γ.altItr s) j φ) :
+    Hierarchy Γ (j + s) (Polarity.quantItr Γ s φ) := by
+  induction s generalizing n j with
+  | zero => simpa using h
+  | succ s ih =>
+    rw [Polarity.altItr_succ] at h
+    rw [Polarity.quantItr_succ, (show j + (s + 1) = (j + 1) + s by omega)]
+    rcases hΓ : Γ.altItr s with _ | _
+    · apply ih
+      rw [hΓ] at h ⊢
+      exact h.sigma
+    · apply ih
+      rw [hΓ] at h ⊢
+      exact h.pi
+
 end Hierarchy
 
 section LOR
