Foundation/FirstOrder/Arithmetic/Basic/Model.lean
@@ -80,6 +80,29 @@ lemma complete (T : ArithmeticTheory) [𝗘𝗤 ℒₒᵣ ⪯ T] (φ : Arithmeti
   rcases standardModel_unique M s
   exact H M
 
+lemma provable_iff_of_models_iff {T : ArithmeticTheory} [𝗘𝗤 ℒₒᵣ ⪯ T] {n}
+    {φ ψ : ArithmeticSemisentence n}
+    (h : ∀ (V : Type) [ORingStructure V] [V↓[ℒₒᵣ] ⊧* T] (e : Fin n → V),
+      V ⊧/e φ ↔ V ⊧/e ψ) :
+    T ⊢ ∀¹* (φ 🡘 ψ) := by
+  apply Arithmetic.complete T _
+  intro V _ _
+  simpa [models_iff] using h V
+
+lemma models_iff_of_provable_iff {T : ArithmeticTheory} [𝗘𝗤 ℒₒᵣ ⪯ T] {n}
+    {φ ψ : ArithmeticSemisentence n} (h : T ⊢ ∀¹* (φ 🡘 ψ)) (V : Type*)
+    [ORingStructure V] [V↓[ℒₒᵣ] ⊧* T] (e : Fin n → V) :
+    V ⊧/e φ ↔ V ⊧/e ψ := by
+  have h' := consequence_iff.mp (Theory.Proof.sound h) V inferInstance
+  simp only [models_iff, Semiformula.eval_allClosure] at h'
+  simpa using h' e
+
+lemma models_iff_of_provable_iff' {T : ArithmeticTheory} [𝗘𝗤 ℒₒᵣ ⪯ T] {n}
+    {φ ψ : ArithmeticSemisentence n} (h : T ⊢ ∀¹* (φ 🡘 ψ)) :
+    ∀ (V : Type) [ORingStructure V] [V↓[ℒₒᵣ] ⊧* T] (e : Fin n → V),
+      V ⊧/e φ ↔ V ⊧/e ψ :=
+  models_iff_of_provable_iff h
+
 lemma weakerThan_of_models (T S : ArithmeticTheory) [𝗘𝗤 ℒₒᵣ ⪯ S]
     (H : ∀ (M : Type*)
            [ORingStructure M]
