Foundation/FirstOrder/Arithmetic/PA/Prenex.lean
@@ -18,15 +18,15 @@ namespace LO.FirstOrder.Arithmetic.Peano
 
 variable {Γ : Polarity} {s n : ℕ}
 
-lemma nonempty_prenexEquivOf {φ : ArithmeticSemisentence n} (h : Hierarchy Γ s φ) :
-    Nonempty (PrenexEquivOf 𝗣𝗔 Γ s _ φ) :=
-  Arithmetic.nonempty_prenexEquivOf h
+lemma nonempty_prenexNormalForm {φ : ArithmeticSemisentence n} (h : Hierarchy Γ s φ) :
+    Nonempty (ArithmeticSemisentence.PrenexNormalForm 𝗣𝗔 Γ s φ) :=
+  Arithmetic.nonempty_prenexNormalForm h
 
 lemma exists_matrix_provable {φ : ArithmeticSemisentence n} (h : Hierarchy Γ s φ) :
     ∃ φ₀ : ArithmeticSemisentence (n + s),
       Hierarchy 𝚺 0 φ₀ ∧ 𝗣𝗔 ⊢ ∀¹* (φ 🡘 Polarity.quantItr Γ s φ₀) := by
-  obtain ⟨φ'⟩ := nonempty_prenexEquivOf h;
-  exact ⟨φ'.matrix, φ'.toPrenex.matrix_Δ₀, φ'.provable⟩
+  obtain ⟨φ'⟩ := nonempty_prenexNormalForm h;
+  exact ⟨φ'.matrix, φ'.matrix_Δ₀, φ'.provable⟩
 
 lemma exists_matrix_provable_of_sentence {σ : ArithmeticSentence} (h : Hierarchy Γ s σ) :
     ∃ π₀ : ArithmeticSemisentence (0 + s),
@@ -35,12 +35,12 @@ lemma exists_matrix_provable_of_sentence {σ : ArithmeticSentence} (h : Hierarch
 
 lemma exists_hierarchy_provable_of_sentence {σ : ArithmeticSentence} (h : Hierarchy 𝚺 (s + 1) σ) :
     ∃ θ : ArithmeticSemisentence 1, Hierarchy 𝚷 s θ ∧ 𝗣𝗔 ⊢ σ 🡘 ∃¹ θ := by
-  obtain ⟨σ'⟩ := nonempty_prenexEquivOf h;
+  obtain ⟨σ'⟩ := nonempty_prenexNormalForm h;
   exact ⟨↑σ'.sigmaInv, σ'.sigmaInv.hierarchy, σ'.provable_sigmaInv⟩
 
 lemma exists_hierarchy_provable_of_sentence_pi {σ : ArithmeticSentence} (h : Hierarchy 𝚷 (s + 1) σ) :
     ∃ θ : ArithmeticSemisentence 1, Hierarchy 𝚺 s θ ∧ 𝗣𝗔 ⊢ σ 🡘 ∀¹ θ := by
-  obtain ⟨σ'⟩ := nonempty_prenexEquivOf h;
+  obtain ⟨σ'⟩ := nonempty_prenexNormalForm h;
   exact ⟨↑σ'.piInv, σ'.piInv.hierarchy, σ'.provable_piInv⟩
 
 end LO.FirstOrder.Arithmetic.Peano
